theories/tests/proofmode.v
@@ -190,6 +190,12 @@ Lemma test_iFrame_persistent (P Q : uPred M) :
   □ P -∗ Q -∗ □ (P ∗ P) ∗ (P ∧ Q ∨ Q).
 Proof. iIntros "#HP". iFrame "HP". iIntros "$". Qed.
 
+Lemma test_iFrame_later_1 P Q : P ∗ ▷ Q -∗ ▷ (P ∗ ▷ Q).
+Proof. iIntros "H". iFrame "H". Qed.
+
+Lemma test_iFrame_later_2 P Q : ▷ P ∗ ▷ Q -∗ ▷ (▷ P ∗ ▷ Q).
+Proof. iIntros "H". iFrame "H". Qed.
+
 Lemma test_iSplit_persistently P Q : □ P -∗ □ (P ∗ P).
 Proof. iIntros "#?". by iSplit. Qed.
 
